@prefix : <http://purl.org/lis590od/Fall17/ExOffenderEmp#> .
@prefix owl: <http://www.w3.org/2002/07/owl#> .
@prefix rdf: <http://www.w3.org/1999/02/22-rdf-syntax-ns#> .
@prefix xml: <http://www.w3.org/XML/1998/namespace> .
@prefix xsd: <http://www.w3.org/2001/XMLSchema#> .
@prefix rdfs: <http://www.w3.org/2000/01/rdf-schema#> .
@base <http://purl.org/lis590od/Fall17/ExOffenderEmp> .

<http://purl.org/lis590od/Fall17/ExOffenderEmp> rdf:type owl:Ontology .

#################################################################
#    Object Properties
#################################################################

###  http://purl.org/lis590od/Fall17/ExOffenderEmp#Had_Previous_Education_Field
:Had_Previous_Education_Field rdf:type owl:ObjectProperty ;
                              rdfs:domain :Prisoner ;
                              rdfs:range :Education_Field ;
                              rdfs:comment "Indicate which education field that the prisoner had before." .


###  http://purl.org/lis590od/Fall17/ExOffenderEmp#Had_Previous_Education_Level
:Had_Previous_Education_Level rdf:type owl:ObjectProperty ;
                              rdfs:domain :Prisoner ;
                              rdfs:range :Education_Level ;
                              rdfs:comment "Indicate which education level that the prisoner had before." .


###  http://purl.org/lis590od/Fall17/ExOffenderEmp#Had_Previous_Occupation
:Had_Previous_Occupation rdf:type owl:ObjectProperty ;
                         rdfs:domain :Prisoner ;
                         rdfs:range :Occupation ;
                         rdfs:comment "Indicate which occupation that the prisoner had before." .


###  http://purl.org/lis590od/Fall17/ExOffenderEmp#Is_Created_By
:Is_Created_By rdf:type owl:ObjectProperty ;
               rdfs:domain :Ex-offender_Employment_Reference ;
               rdfs:range :Employment_Agency ;
               rdfs:comment "To identify the employment angency who creates/files the employment reference" .


###  http://purl.org/lis590od/Fall17/ExOffenderEmp#Is_Created_For
:Is_Created_For rdf:type owl:ObjectProperty ;
                rdfs:domain :Ex-offender_Employment_Reference ;
                rdfs:range :Prisoner ;
                rdfs:comment "Mapping between the reference document to the prisoner" .


###  http://purl.org/lis590od/Fall17/ExOffenderEmp#Is_Referred_By
:Is_Referred_By rdf:type owl:ObjectProperty ;
                rdfs:domain :Prisoner ;
                rdfs:range :Employment_Agency ;
                rdfs:comment "Identify the angency who takes responsibility to refer the prisoner to an employment opportunity." .


###  http://purl.org/lis590od/Fall17/ExOffenderEmp#Manage
:Manage rdf:type owl:ObjectProperty ;
        rdfs:domain :Employment_Agency ;
        rdfs:range :Employment_Opportunity ;
        rdfs:comment "To identify which employment agency manage which employment opportunities. An agency could be responsible for multiple employment opportunities." .


###  http://purl.org/lis590od/Fall17/ExOffenderEmp#Refer_To
:Refer_To rdf:type owl:ObjectProperty ;
          rdfs:domain :Ex-offender_Employment_Reference ;
          rdfs:range :Employment_Opportunity ;
          rdfs:comment "Mapping between a reference document to the corrsponding employment opportunity." .


###  http://purl.org/lis590od/Fall17/ExOffenderEmp#Refer_To_Occupation
:Refer_To_Occupation rdf:type owl:ObjectProperty ;
                     rdfs:domain :Employment_Opportunity ;
                     rdfs:range :Occupation ;
                     rdfs:comment "Indicate the occupation that the employment opportunity refers to." .


###  http://purl.org/lis590od/Fall17/ExOffenderEmp#Require
:Require rdf:type owl:ObjectProperty ;
         rdfs:domain :Employment_Opportunity ;
         rdfs:range :Education_Field ,
                    :Education_Level ;
         rdfs:comment "Indicate which requirements that the employment opportunity has, including educational field and level." .


#################################################################
#    Data properties
#################################################################

###  http://purl.org/lis590od/Fall17/ExOffenderEmp#Age
:Age rdf:type owl:DatatypeProperty ;
     rdfs:domain :Prisoner ;
     rdfs:comment "Age of the prisoner." .


###  http://purl.org/lis590od/Fall17/ExOffenderEmp#Document_ID
:Document_ID rdf:type owl:DatatypeProperty ;
             rdfs:domain :Ex-offender_Employment_Reference ;
             rdfs:comment "Reference Document ID. Each document is equipvalent to one prisoner and one opportunity only." .


###  http://purl.org/lis590od/Fall17/ExOffenderEmp#Duration_Left_In_Prison
:Duration_Left_In_Prison rdf:type owl:DatatypeProperty ;
                         rdfs:domain :Prisoner ;
                         rdfs:comment "Indicate how long does the prisoner have to stay in the prison. This is a dynamic value (change and updated overtime)" .


###  http://purl.org/lis590od/Fall17/ExOffenderEmp#Name
:Name rdf:type owl:DatatypeProperty ;
      rdfs:domain :Prisoner ;
      rdfs:comment "Name of the prisoner" .


#################################################################
#    Classes
#################################################################

###  http://purl.org/lis590od/Fall17/ExOffenderEmp#Education_Field
:Education_Field rdf:type owl:Class ;
                 rdfs:comment "Indicate which field the ex-offender graduated from before." .


###  http://purl.org/lis590od/Fall17/ExOffenderEmp#Education_Level
:Education_Level rdf:type owl:Class ;
                 rdfs:comment "Indicate level of education that the ex-offender have. Such as: High School, Bachelor Degree, Master Degree, etc." .


###  http://purl.org/lis590od/Fall17/ExOffenderEmp#Employment_Agency
:Employment_Agency rdf:type owl:Class ;
                   rdfs:comment "Indicate the agency who is responsible for the employment reference." .


###  http://purl.org/lis590od/Fall17/ExOffenderEmp#Employment_Opportunity
:Employment_Opportunity rdf:type owl:Class ;
                        rdfs:comment "Indicate the employment opportunity, including informatuon about the opportunity" .


###  http://purl.org/lis590od/Fall17/ExOffenderEmp#Ex-offender_Employment_Reference
:Ex-offender_Employment_Reference rdf:type owl:Class ;
                                  rdfs:comment "The document contains information about the ex-offender who is referred, which employment opportunity refers to, who is the agency that responsible." .


###  http://purl.org/lis590od/Fall17/ExOffenderEmp#Occupation
:Occupation rdf:type owl:Class ;
            rdfs:comment "Indicate the previous occupation that the ex-offender had." .


###  http://purl.org/lis590od/Fall17/ExOffenderEmp#Prisoner
:Prisoner rdf:type owl:Class ;
          rdfs:comment "Information about the person who is in prison by the time they are enrolled the ex-offender employment reference system." .


###  Generated by the OWL API (version 4.2.8.20170104-2310) https://github.com/owlcs/owlapi
